\documentclass[../main.tex]{subfiles}
\begin{document}

\subsubsection{Map}

The $map$ operation accepts the following arguments

\begin{itemize}
\item Operation or Primitive
\item A Collection
\item Additional Arguments passed to the Operator or Primitive
\end{itemize}
and returns a collection of Operation $Operation(x_{n}, args) \ \lor Primitive(x_{n}, args)$ respectively
$\\\\$
Given an input Collection $X$ and a Operation $o$ or Primitive $p$ where
$$X = <x_{i}..x_{n}..x_{j}>$$
and that collection consists of one or more members $x_{n}$ within the range $i..j$
$$i \leq n \leq j  \implies i \prec n \prec j \iff i \not= n \not= j$$
then
$$map(o, \ X, \ args) = Y \ \land \ map(p, \ X, \ args) = Y'$$
such that
$$Y = <o(x_{i}, args)..o(x_{n}, args)..o(x_{j}, args)>$$
and
$$Y' = <p(x_{i}, args)..p(x_{n}, args)..p(x_{j}, args)>$$
which establishes both $Y$ and $Y'$ are a Collection where each member $y_{n}$ or $y'_{n}$ is the result of passing $x_{n}$ and $args$ to $o$ or $p$ respectively.

$\\$
In otherwords
$$o(x_{i}, args) \mapsto y_{i} \land o(x_{n}, args) \mapsto y_{n} \land o(x_{j}, args) \mapsto y_{j}$$
$$p(x_{i}, args) \mapsto y'_{i} \land p(x_{n}, args) \mapsto y'_{n} \land p(x_{j}, args) \mapsto y'_{j}$$
which implies both collections $Y$ and $Y'$ have the same ordering as collection $X$
$$ i_{o(x, args)} = i_{y} \ \land \ n_{o(x, args)} = n_{y} \ \land \ j_{o(x, args)} = j_{y} $$
$$ i_{p(x, args)} = i_{y'} \ \land \ n_{p(x, args)} = n_{y'} \ \land \ j_{p(x, args)} = j_{y'}$$
When $X$ contains non-distinct values, $o$ and $p$ are unaffected.
$$o(x_{n}, args) = y_{n}$$
$$o(x_{n'}, args) = y_{n'}$$
$$o(x_{n' + 1}, args) = y_{n'}$$
$$\iff$$
$$x_{n'} \equiv x_{n'+1} \land x_{n'} \not \equiv x_{n}$$
$$\implies $$
$$x_{n} \not \equiv  x_{n' + 1}$$
$$\implies $$
$$o(x_{n'}, args) = o(x_{n' + 1}, args) \not= o(x_{n}, args)$$
Because $p$ is just a composition of $o$'s, the same property holds for primitives
$$p(x_{n}, args) = y'_{n}$$
$$p(x_{n'}, args) = y'_{n'}$$
$$p(x_{n' + 1}, args) = y'_{n'}$$
$$\iff$$
$$x_{n'} \equiv x_{n'+1} \land x_{n'} \not \equiv x_{n}$$
$$\implies $$
$$x_{n} \not \equiv  x_{n' + 1}$$
$$\implies $$
$$p(x_{n'}, args) = p(x_{n' + 1}, args) \not= p(x_{n}, args)$$
\end{document}
